src/3d/prelude/EverParse3d.Prelude.fsti
@@ -713,11 +713,11 @@ let cast_mul_fits_32_64 (x y :U32.t)
 val in_codomain #nz #wk (#k: parser_kind nz wk) #t (p: parser k t) (x: t) : prop
 val serialize #nz #wk (#k: parser_kind nz wk) #t (p: parser k t) (x: t { in_codomain p x }) : GTot (Seq.seq U8.t)
 
-let serialized_fits #nz #wk (#k: parser_kind nz wk) #t (p: parser k t) (x: t) (sz: nat) : prop =
+let serialized_fits #nz #wk (#k: parser_kind nz wk) #t (p: parser k t) (x: t) (sz: int) : prop =
   in_codomain p x /\ Seq.length (serialize p x) <= sz
 
+inline_for_extraction
 let pulse_ser_t #nz #wk #k (#t:Type0) (p: parser #nz #wk k t) (x: erased t) (frame: vprop) : Type0 =
-
   arr: PA.array FStar.UInt8.t {SZ.fits (PA.length arr)} ->
   i: SZ.t { SZ.v i <= PA.length arr /\ serialized_fits p x (PA.length arr - SZ.v i) } ->
   stt SZ.t
@@ -764,3 +764,7 @@ val all_bytes_pulse_to_all_bytes : all_bytes_pulse -> GTot all_bytes
 val all_bytes_pulse_match : all_bytes -> all_bytes_pulse -> vprop
 val pulse_ser_all_bytes (h: erased all_bytes) (l: all_bytes_pulse) :
   pulse_ser_t parse_all_bytes h (all_bytes_pulse_match h l)
+
+val all_zeros_pulse_to_all_zeros : SizeT.t -> GTot all_zeros
+val pulse_ser_all_zeros (h: erased all_zeros) (l: SizeT.t) :
+  pulse_ser_t parse_all_zeros h (pure (all_zeros_pulse_to_all_zeros l == reveal h))
